theories/Core/ITreeMonad.v
@@ -5,7 +5,6 @@
 
 From ITree Require Import
      Basics.Basics
-     Basics.Monad
      Core.ITreeDefinition
      Eq.Eqit
      Eq.UpToTaus.
@@ -26,14 +25,12 @@ Instance MonadLawsE_ITree {E} : MonadLawsE (itree E).
 Proof.
   constructor.
   - intros a b f x.
-    unfold Monad.bind, Monad.ret, Monad_itree.
-    unfold eq1, Eq1_ITree. rewrite bind_ret_l. reflexivity.
-  - intros a x.    unfold Monad.bind, Monad.ret, Monad_itree.
-    unfold eq1, Eq1_ITree. rewrite bind_ret_r. reflexivity.
-  - intros a b c x f g. unfold Monad.bind, Monad.ret, Monad_itree.
-    unfold eq1, Eq1_ITree. rewrite bind_bind. reflexivity.
-  - unfold Monad.bind, Monad_itree.
-    intros.
+    by setoid_rewrite bind_ret_l.
+  - intros a x.
+    by setoid_rewrite bind_ret_r.
+  - intros a b c x f g.
+    by setoid_rewrite bind_bind.
+  - intros.
     repeat red.
     intros.
     apply eqit_bind; auto.
