theories/Core/KTreeFacts.v
@@ -31,7 +31,6 @@ Local Open Scope cat_scope.
 
 Ltac unfold_ktree :=
   unfold
-    Monad.eq1, Eq1_ITree,
     Basics.iter, MonadIter_itree,
     assoc_l, AssocL_Coproduct,
     bimap, Bimap_Coproduct,
@@ -139,7 +138,6 @@ Qed.
           (iter (C := ktree E)).
 Proof.
   intros body1 body2 EQ_BODY a. repeat red in EQ_BODY.
-  unfold_ktree.
   eapply (eq_itree_iter' eq); auto.
   intros; eapply eqit_mon, EQ_BODY; auto.
   intros [] _ []; auto; econstructor; subst; auto.
@@ -151,7 +149,6 @@ Qed.
           (iter (C := ktree E)).
 Proof.
   intros body1 body2 EQ_BODY a. repeat red in EQ_BODY.
-  unfold_ktree.
   eapply (eutt_iter' eq); auto.
   intros ? _ []; eapply eqit_mon, EQ_BODY; auto.
   intros [] _ []; auto; econstructor; auto.
@@ -188,22 +185,23 @@ Qed.
 
 #[global] Instance IterUnfold_ktree {E} : IterUnfold (ktree E) sum.
 Proof.
-  repeat intro. unfold_ktree. rewrite unfold_iter_ktree.
+  repeat intro. rewrite unfold_iter_ktree.
   eapply eutt_clo_bind; try reflexivity.
   intros [] ? []; try rewrite tau_eutt; reflexivity.
 Qed.
 
 #[global] Instance IterNatural_ktree {E} : IterNatural (ktree E) sum.
 Proof.
-  repeat intro. unfold_ktree.
+  repeat intro.
   revert a0.
   einit. ecofix CIH. intros.
+  unfold_ktree.
   rewrite 2 unfold_iter_ktree.
-  rewrite !bind_bind.
+  repeat setoid_rewrite bind_bind.
   ebind; econstructor; try reflexivity.
   intros [] ? [].
-  - rewrite bind_tau, 2 bind_ret_l. etau.
-  - rewrite bind_ret_l, !bind_bind. setoid_rewrite bind_ret_l. rewrite bind_ret_r.
+  - setoid_rewrite bind_tau. do 2 setoid_rewrite bind_ret_l. etau.
+  - setoid_rewrite bind_ret_l; repeat setoid_rewrite bind_bind. setoid_rewrite bind_ret_l. rewrite bind_ret_r.
     reflexivity.
 Qed.
 
@@ -328,11 +326,23 @@ Proof.
 Qed.
 
 (* Equation merging the sequence of two [iter] into one *)
-Lemma cat_iter: 
-  forall {E: Type -> Type} {a b c} (f: ktree E a (a + b)) (g: ktree E b (b + c)), 
+Lemma cat_iter:
+  forall {E: Type -> Type} {a b c} (f: ktree E a (a + b)) (g: ktree E b (b + c)),
     ITree.iter f >>> ITree.iter g ⩯ inl_ >>> ITree.iter (case_ (f >>> inl_) (g >>> inr_ >>> assoc_l)).
 Proof.
   intros *.
+  unfold
+    Basics.iter, MonadIter_itree,
+    assoc_l, AssocL_Coproduct,
+    bimap, Bimap_Coproduct,
+    cat, Cat_Kleisli, inl_, Inl_Kleisli, inr_, Inr_Kleisli, case_, Case_Kleisli, case_sum,
+    lift_ktree_.
+  cbn.
+  Unset Printing Notations.
+  simpl.
+  cbn.
+
+
   unfold_ktree.
   (* We move to the eworld *)
   einit.
@@ -342,36 +352,38 @@ Proof.
   ecofix CIH.
   intros.
   cbn.
-  rewrite bind_ret_l.
+  setoid_rewrite bind_ret_l.
   (* We unfold one step on both sides *)
   match goal with
   |- euttG _ _ _ _ _ ?t _ => remember t; rewrite unfold_iter; subst
   end.
   rewrite unfold_iter; cbn.
-  rewrite !bind_bind.
+  repeat setoid_rewrite bind_bind.
   ebind.
   (* We run f a first time on both side *)
   econstructor; [reflexivity | intros [xa | xb] ? <-].
   - (* If we loop back to f, we can conclude by coinduction *)
-    rewrite ! bind_ret_l.
+    repeat setoid_rewrite bind_ret_l.
     rewrite bind_tau.
     etau.
     specialize (CIHL xa). cbn in CIHL.
     match goal with
       |- euttG _ _ _ _ _ ?t _ => remember t
     end.
+    clear CIHH.
     rewrite <- bind_ret_l.
     ebase.
+    right. apply CIHL.
   - (* If we exit the first loop *)
-    rewrite ! bind_ret_l.
+    setoid_rewrite bind_ret_l.
     (* We setup a second coinductive point in the simulation.
        We just make sure to first get rid of the additional tau guard
-       that we have encountered in the right of the equation to keep the second part clean. 
+       that we have encountered in the right of the equation to keep the second part clean.
      *)
     rewrite tau_euttge.
     generalize xb.
     ecofix CIH'.
-    
+
     intros ?.
     (* We unfold a new step of computation *)
     rewrite unfold_iter; cbn.
